@prefix dc: <http://purl.org/dc/terms/> .
@prefix dcterms: <http://purl.org/dc/terms/> .
@prefix rdf: <http://www.w3.org/1999/02/22-rdf-syntax-ns#> .
@prefix rdfs: <http://www.w3.org/2000/01/rdf-schema#> .
@prefix schema: <http://schema.org/> .
@prefix xml: <http://www.w3.org/XML/1998/namespace> .
@prefix xsd: <http://www.w3.org/2001/XMLSchema#> .
@prefix owl: <http://www.w3.org/2002/07/owl#> .
@prefix saref: <https://w3id.org/saref#> .
@prefix bigiot: <http://big-iot.eu/core#> .

schema:BasicData a rdfs:Class ;
    rdfs:label "Basic data types" ;
    dc:source <http://vocab.datex.org/terms#BasicData> ;
    rdfs:comment "Data that is either measured or calculated (elaborated) at the same time or over the same time period. " ;
    rdfs:subClassOf schema:QuantitativeValue .

schema:SmartBuilding a rdfs:Class ;
    rdfs:label "A class of categories for Smart Building offerings" ;
    rdfs:comment "A smart building category class." ;
    rdfs:subClassOf schema:Enumeration .

schema:smartBuilding a schema:SmartBuilding ;
    rdfs:label "A category for smart building offerings" ;
    rdfs:comment "A sub-category of SmartBuilding." .

schema:smartHome a schema:SmartBuilding ;
    rdfs:label "A category for smart Home offerings" ;
    rdfs:comment "A sub-category of SmartBuilding to categorize the offerings relating to smart home." .

schema:smartOffice a schema:SmartBuilding ;
    rdfs:label "A category for smart Office offerings" ;
    rdfs:comment "A sub-category of SmartBuilding to categorize the offerings relating to smart office." .
	
schema:Switch a rdfs:Class ;
    rdfs:label "A light switch" ;
    rdfs:comment "A light switch." ;
    rdfs:subClassOf saref:LightSwitch .
	
schema:trigger a rdf:Property ;
    rdfs:label "trigger" ;
    schema:domainIncludes schema:Switch ;
    schema:rangeIncludes schema:Number ;
    rdfs:comment "trigger the execution of an offering" .	
	
schema:Light a rdfs:Class ;
    rdfs:label "A light device" ;
    rdfs:comment "A light device." ;
    rdfs:subClassOf saref:Light .
	
schema:status a rdf:Property ;
    rdfs:label "Status" ;
    schema:domainIncludes schema:Light ;
	schema:domainIncludes schema:Switch ;
	schema:rangeIncludes schema:Text ;
    rdfs:comment "On or off status" .		

schema:switchCat
        a                schema:SmartBuilding , schema:smartBuilding ;
        rdfs:comment     "A switch device - subcategory of schema:smartOffice." ;
        rdfs:label       "A switch device" ;
        bigiot:refersTo  schema:Switch .

schema:lightCat
        a                schema:SmartBuilding , schema:smartBuilding ;
        rdfs:comment     "A light device - subcategory of schema:smartOffice." ;
        rdfs:label       "A light device" ;
        bigiot:refersTo  schema:Light .


